start proof

sppf/sppf.v
@@ -1,7 +1,6 @@
 Import Nat.
 
-Add LoadPath "..".
-Require Import CFG.Definitions.
+Require Import List.
 
 Module Base.
 
@@ -15,7 +14,7 @@ Module Base.
   | mk_nonterminal_node : Vt  -> nat -> nat -> SPPF_node
   | mk_intermediate_node :  @phrase Tt Vt -> nat -> nat -> SPPF_node.
 
-  Inductive valid_parent : SPPF_node -> Prop :=
+  Inductive valid_parent : SPPF_node -> Type :=
   | mk_nonterminal_node_parent v from to : valid_parent (mk_nonterminal_node v from to)
   | mk_intermediate_node_parent p from to : valid_parent (mk_intermediate_node p from to).
 
@@ -26,18 +25,148 @@ Module Base.
   Inductive SPPF_rel : Type :=
   | mk_rel : forall p : SPPF_node, (valid_parent p) -> packed_SPPF_node -> SPPF_rel.
 
-  Record SPPF := mkSPPF {
-    relations : list SPPF_rel;
-  }.
+  Definition SPPF := list SPPF_rel.
 
   Inductive sppf_der (sppf: SPPF) :  SPPF_node -> word -> Prop :=
   |  terDer (t : Tt) (from : nat) (to : nat) : sppf_der sppf (mk_terminal_node t from to) [T t]
   |  epsilonDer (from : nat) (to : nat) : sppf_der sppf (mk_epsilon_node from to) []
-  |  mkRel1 p vp ch1 w1 : In (mk_rel p vp (mk_packed_node1 ch1)) (relations sppf) ->
+  |  mkRel1 p vp ch1 w1 : In (mk_rel p vp (mk_packed_node1 ch1)) sppf ->
                           (sppf_der sppf ch1 w1) -> sppf_der sppf p w1
-  |  mkRel2 p vp ch1 ch2 w1 w2 : In (mk_rel p vp (mk_packed_node2 ch1 ch2)) (relations sppf) ->
-                          (sppf_der sppf ch1 w1) -> (sppf_der sppf ch2 w2) -> sppf_der sppf p w1.
+  |  mkRel2 p vp ch1 ch2 w1 w2 : In (mk_rel p vp (mk_packed_node2 ch1 ch2)) sppf ->
+                                 (sppf_der sppf ch1 w1) -> (sppf_der sppf ch2 w2) -> sppf_der sppf p w1.
 
+  Inductive triple :=
+    mkTriple : nat -> (@phrase Tt Vt) -> nat -> triple.
+
+  Definition valid_parent_to_triple (s : SPPF_node) (vp : (valid_parent s)) : triple  :=
+    match vp with
+    | mk_nonterminal_node_parent v from to => (mkTriple from [Vs (V v)] to)
+    | mk_intermediate_node_parent p from to => (mkTriple from p to)
+    end.
+
+  Definition node_to_phrase (s : SPPF_node) : (@phrase Tt triple):=
+    match s with
+    | mk_terminal_node t from to => [Ts (T t)]
+    | mk_epsilon_node from to  => []
+    | mk_nonterminal_node v from to => [Vs (V (mkTriple from [Vs (V v)] to))]
+    | mk_intermediate_node p from to => [Vs (V (mkTriple from p to))]
+    end.
+
+  Definition SPPF_rel_to_rule (r : SPPF_rel) : (@rule Tt triple) :=
+    match r with
+    |  mk_rel p v n => let var := V (valid_parent_to_triple p v) in
+                       match n with
+                       | mk_packed_node1 n1 => R var (node_to_phrase n1)
+                       | mk_packed_node2 n1 n2 => R var ((node_to_phrase n1) ++ (node_to_phrase n2))
+                       end
+    end.
+
+  Definition SPPF_to_grammar (s : SPPF) : (@grammar Tt triple) :=
+    map SPPF_rel_to_rule s.
+
+
+  Theorem in_p_eq (p : SPPF_node) (is_p1 is_p2 : valid_parent p) :
+    (valid_parent_to_triple p is_p1 = valid_parent_to_triple p is_p2).
+  Proof.
+    destruct is_p1.
+    simpl.
+    remember (mk_nonterminal_node v from to) as p in *.
+    destruct is_p2.
+    injection Heqp.
+    clear Heqp.
+    intro H0; rewrite H0 in *; clear H0.
+    intro H0; rewrite H0 in *; clear H0.
+    intro H0; rewrite H0 in *; clear H0.
+    simpl.
+    reflexivity.
+    discriminate.
+    simpl.
+    remember (mk_intermediate_node p from to) as n in *.
+    destruct is_p2.
+    discriminate.
+    injection Heqn.
+    clear Heqn.
+    intro H0; rewrite H0 in *; clear H0.
+    intro H0; rewrite H0 in *; clear H0.
+    intro H0; rewrite H0 in *; clear H0.
+    simpl.
+    reflexivity.
+  Qed.
+
+  Theorem in1 (t : Tt) (from to : nat) (p : SPPF_node) (is_p vp : valid_parent p) (sppf : SPPF) :
+    In (mk_rel p vp (mk_packed_node1 (mk_terminal_node t from to))) sppf ->
+    In (R (V (valid_parent_to_triple p is_p)) (to_phrase [T t])) (SPPF_to_grammar sppf).
+  Proof.
+    intro H0.
+    induction sppf.
+    contradiction.
+    destruct H0.
+    simpl.
+    left.
+    rewrite H.
+    simpl.
+    assert (Heq : (valid_parent_to_triple p vp) = (valid_parent_to_triple p is_p)).
+    apply in_p_eq.
+    rewrite Heq.
+    reflexivity.
+    right.
+    apply IHsppf.
+    exact H.
+  Qed.
+
+  Theorem in2 (from to : nat) (p : SPPF_node) (is_p vp : valid_parent p) (sppf : SPPF) :
+    In (mk_rel p vp (mk_packed_node1 (mk_epsilon_node from to))) sppf ->
+    In (R (V (valid_parent_to_triple p is_p)) (to_phrase [])) (SPPF_to_grammar sppf).
+  Proof.
+    intro H0.
+    induction sppf.
+    contradiction.
+    destruct H0.
+    left.
+    rewrite H.
+    simpl.
+    assert (Heq : (valid_parent_to_triple p vp) = (valid_parent_to_triple p is_p)).
+    apply in_p_eq.
+    rewrite Heq.
+    reflexivity.
+    right.
+    apply IHsppf.
+    exact H.
+  Qed.
+
+  Theorem trains1 (sppf : SPPF) (n : SPPF_node) (is_p : valid_parent n) (w : word)
+           (d : (sppf_der sppf n w)) :
+    der (SPPF_to_grammar sppf) (V (valid_parent_to_triple n is_p)) (to_phrase w).
+  Proof.
+    induction d.
+    remember (mk_terminal_node t from to) as root in *.
+    destruct is_p; discriminate.
+    remember (mk_epsilon_node from to) as root in *.
+    destruct is_p; discriminate.
+    destruct ch1.
+    remember (mk_terminal_node t n n0) as root in *.
+    destruct d.
+    injection Heqroot.
+    clear Heqroot.
+    intro H0; rewrite H0 in *; clear H0.
+    intro H0; rewrite H0 in *; clear H0.
+    intro H0; rewrite H0 in *; clear H0.
+
+    apply rDer.
+    apply (in1 t n n0 p is_p vp).
+    exact H.
+
+    apply rDer.
+
+    apply (in2 from to p is_p vp).
+    exact H.
+
+    rewrite -> Heqroot in IHd.
+    simpl IHd.
+    assert der (SPPF_to_grammar sppf) ((mkTriple n [Vs (V v)] n0)) (to_phrase w1).
+
+
+    apply IHd.
 
 End Base.
 
